Add support for Z*Z casts, get montred working

src/Experiments/SimplyTypedArithmetic.v
@@ -2021,6 +2021,7 @@ Module Compilers.
           | Z_zselect : ident (Z * Z * Z) Z
           | Z_add_modulo : ident (Z * Z * Z) Z
           | Z_cast (range : zrange) : ident Z Z
+          | Z_cast2 (range : zrange * zrange) : ident (Z * Z) (Z * Z)
           .
 
           Notation curry0 f
@@ -2042,6 +2043,11 @@ Module Compilers.
 
           Section gen.
             Context (cast_outside_of_range : zrange -> BinInt.Z -> BinInt.Z).
+
+            Definition cast (r : zrange) (x : BinInt.Z)
+              := if (lower r <=? x) && (x <=? upper r)
+                 then x
+                 else cast_outside_of_range r x.
 
             (** Interpret identifiers where the behavior of [Z_cast]
                 on a value that does not fit in the range is given by
@@ -2089,9 +2095,8 @@ Module Compilers.
                  | Z_sub_get_borrow_concrete s => curry2 (Z.sub_get_borrow s)
                  | Z_zselect => curry3 Z.zselect
                  | Z_add_modulo => curry3 Z.add_modulo
-                 | Z_cast r => fun x => if (lower r <=? x) && (x <=? upper r)
-                                        then x
-                                        else cast_outside_of_range r x
+                 | Z_cast r => cast r
+                 | Z_cast2 (r1, r2) => fun '(x1, x2) => (cast r1 x1, cast r2 x2)
                  end.
           End gen.
 
@@ -2229,6 +2234,7 @@ Module Compilers.
             Notation zselect := Z_zselect.
             Notation add_modulo := Z_add_modulo.
             Notation cast := Z_cast.
+            Notation cast2 := Z_cast2.
           End Z.
 
           Module Nat.
@@ -2632,6 +2638,16 @@ Module Compilers.
          | Some (existT s (idc, args))
            => match idc in ident s t return expr s -> option (zrange * expr type.Z) with
               | ident.Z_cast r => fun v => Some (r, v)
+              | _ => fun _ => None
+              end args
+         | None => None
+         end.
+
+    Definition invert_Z_cast2 (e : @expr var (type.Z * type.Z)) : option ((zrange * zrange) * @expr var (type.Z * type.Z))
+      := match invert_AppIdent e with
+         | Some (existT s (idc, args))
+           => match idc in ident s t return expr s -> option ((zrange * zrange) * expr (type.Z * type.Z)) with
+              | ident.Z_cast2 r => fun v => Some (r, v)
               | _ => fun _ => None
               end args
          | None => None
@@ -3156,6 +3172,7 @@ Module Compilers.
                   | ident.Z_zselect as idc
                   | ident.Z_add_modulo as idc
                   | ident.Z_cast _ as idc
+                  | ident.Z_cast2 _ as idc
                     => cps_of (Uncurried.expr.default.ident.interp idc)
                   | ident.Z_mul_split_concrete s
                     => cps_of (curry2 (Z.mul_split s))
@@ -3371,6 +3388,7 @@ Module Compilers.
                      (ident.snd @@ (Var xyk))
                        @ ((idc : default.ident _ (type.Z * type.Z))
                             @@ (ident.fst @@ (Var xyk)))
+                | ident.Z_cast2 _ as idc
                 | ident.Z_mul_split_concrete _ as idc
                 | ident.Z_add_get_carry_concrete _ as idc
                 | ident.Z_sub_get_borrow_concrete _ as idc
@@ -3895,14 +3913,14 @@ Module Compilers.
              | type.type_primitive x => primitive.option.interp x
              | type.prod A B => interp A * interp B
              | type.arrow s d => interp s -> interp d
-             | type.list A => list (interp A)
+             | type.list A => option (list (interp A))
              end.
         Fixpoint None {t : type} : interp t
           := match t with
              | type.type_primitive x => @primitive.option.None x
              | type.prod A B => (@None A, @None B)
              | type.arrow s d => fun _ => @None d
-             | type.list A => @nil (interp A)
+             | type.list A => Datatypes.None
              end.
         Fixpoint Some {t : type} : type.interp t -> interp t
           := match t with
@@ -3911,7 +3929,7 @@ Module Compilers.
                => fun x : type.interp A * type.interp B
                   => (@Some A (fst x), @Some B (snd x))
              | type.arrow s d => fun _ _ => @None d
-             | type.list A => List.map (@Some A)
+             | type.list A => fun ls => Datatypes.Some (List.map (@Some A) ls)
              end.
         Fixpoint is_tighter_than {t} : interp t -> interp t -> bool
           := match t with
@@ -3922,7 +3940,13 @@ Module Compilers.
                   => @is_tighter_than A ra ra' && @is_tighter_than B rb rb'
              | type.arrow s d => fun _ _ => false
              | type.list A
-               => fold_andb_map (@is_tighter_than A)
+               => fun ls1 ls2
+                  => match ls1, ls2 with
+                     | Datatypes.None, Datatypes.None => true
+                     | Datatypes.Some _, Datatypes.None => true
+                     | Datatypes.None, Datatypes.Some _ => false
+                     | Datatypes.Some ls1, Datatypes.Some ls2 => fold_andb_map (@is_tighter_than A) ls1 ls2
+                     end
              end.
         Fixpoint is_bounded_by {t} : interp t -> Compilers.type.interp t -> bool
           := match t return interp t -> Compilers.type.interp t -> bool with
@@ -3933,7 +3957,11 @@ Module Compilers.
                   => @is_bounded_by A ra ra' && @is_bounded_by B rb rb'
              | type.arrow s d => fun _ _ => false
              | type.list A
-               => fold_andb_map (@is_bounded_by A)
+               => fun ls1 ls2
+                  => match ls1 with
+                     | Datatypes.None => false
+                     | Datatypes.Some ls1 => fold_andb_map (@is_bounded_by A) ls1 ls2
+                     end
              end.
 
         Lemma is_tighter_than_Some_is_bounded_by {t} r1 r2 val
@@ -3954,7 +3982,10 @@ Module Compilers.
                          | apply conj
                          | Z.ltb_to_lt; omega
                          | rewrite @fold_andb_map_map in * ].
-          { revert r1 r2 val Htight Hbounds IHt.
+          { lazymatch goal with
+            | [ r1 : list (interp t), r2 : list (type.interp t), val : list (Compilers.type.interp t) |- _ ]
+              => revert r1 r2 val Htight Hbounds IHt
+            end; intros r1 r2 val; revert r1 r2 val.
             induction r1, r2, val; cbn; auto with nocore; try congruence; [].
             rewrite !Bool.andb_true_iff; intros; destruct_head'_and; split; eauto with nocore. }
         Qed.
@@ -4000,12 +4031,18 @@ Module Compilers.
              | ident.Z_sub_get_borrow
              | ident.Z_modulo
                => fun _ => type.option.None
-             | ident.nil t => curry0 (@nil (type.option.interp t))
-             | ident.cons t => curry2 (@Datatypes.cons (type.option.interp t))
+             | ident.nil t => curry0 (Some (@nil (type.option.interp t)))
+             | ident.cons t => curry2 (fun a => option_map (@Datatypes.cons (type.option.interp t) a))
              | ident.fst A B => @Datatypes.fst (type.option.interp A) (type.option.interp B)
              | ident.snd A B => @Datatypes.snd (type.option.interp A) (type.option.interp B)
              | ident.List_nth_default_concrete T d n
-               => fun ls => @nth_default (type.option.interp T) type.option.None ls n
+               => fun ls
+                  => match ls with
+                     | Datatypes.Some ls
+                       => @nth_default (type.option.interp T) type.option.None ls n
+                     | Datatypes.None
+                       => type.option.None
+                     end
              | ident.Z_shiftr _ as idc
              | ident.Z_shiftl _ as idc
              | ident.Z_opp as idc
@@ -4029,6 +4066,16 @@ Module Compilers.
                           | Some r => ZRange.intersection r range
                           | None => range
                           end
+             | ident.Z_cast2 (r1, r2)
+               => fun '((r1', r2') : option zrange * option zrange)
+                  => (Some match r1' with
+                           | Some r => ZRange.intersection r r1
+                           | None => r1
+                           end,
+                      Some match r2' with
+                           | Some r => ZRange.intersection r r2
+                           | None => r2
+                           end)
              | ident.Z_mul_split_concrete split_at
                => fun '((x, y) : option zrange * option zrange)
                   => match x, y with
@@ -4110,7 +4157,7 @@ Module Compilers.
   End DefaultValue.
 
   Module partial.
-    Notation Zdata := (option zrange).
+    Notation data := ZRange.type.option.interp.
     Section value.
       Context (var : type -> Type).
       Definition value_prestep (value : type -> Type) (t : type)
@@ -4125,12 +4172,10 @@ Module Compilers.
         := match t return Type with
            | type.arrow _ _ as t
              => value_prestep value t
-           | type.type_primitive type.Z as t
-             => Zdata * @expr var t + value_prestep value t
            | type.prod _ _ as t
            | type.list _ as t
            | type.type_primitive _ as t
-             => @expr var t + value_prestep value t
+             => data t * @expr var t + value_prestep value t
            end%type.
       Fixpoint value (t : type)
         := value_step value t.
@@ -4145,6 +4190,38 @@ Module Compilers.
            | type.arrow s d => fun _ => @value_default d
            | type.list A => inr (@nil (value A))
            end.
+
+      Fixpoint data_from_value {t} : value t -> data t
+        := match t return value t -> data t with
+           | type.arrow _ _ as t
+             => fun _ => ZRange.type.option.None
+           | type.prod A B as t
+             => fun v
+                => match v with
+                   | inl (data, _) => data
+                   | inr (a, b)
+                     => (@data_from_value A a, @data_from_value B b)
+                   end
+           | type.list A as t
+             => fun v
+                => match v with
+                   | inl (data, _) => data
+                   | inr ls
+                     => Some (List.map (@data_from_value A) ls)
+                   end
+           | type.type_primitive type.Z as t
+             => fun v
+                => match v with
+                   | inl (data, _) => data
+                   | inr v => Some r[v~>v]%zrange
+                   end
+           | type.type_primitive _ as t
+             => fun v
+                => match v with
+                   | inl (data, _) => data
+                   | inr _ => ZRange.type.option.None
+                   end
+           end.
     End value.
 
     Module expr.
@@ -4154,9 +4231,19 @@ Module Compilers.
           : value var t -> @expr var t
           := match t return value var t -> expr t with
              | type.prod A B as t
-               => fun x : expr t + value var A * value var B
+               => fun x : (data A * data B) * expr t + value var A * value var B
                   => match x with
-                     | inl v => v
+                     | inl ((da, db), v)
+                       => match A, B return data A -> data B -> expr (A * B) -> expr (A * B) with
+                          | type.Z, type.Z
+                            => fun da db v
+                               => match da, db with
+                                  | Some r1, Some r2
+                                    => (ident.Z.cast2 (r1, r2)%core @@ v)%expr
+                                  | _, _ => v
+                                  end
+                          | _, _ => fun _ _ v => v
+                          end da db v
                      | inr (a, b) => (@reify A a, @reify B b)%expr
                      end
              | type.arrow s d
@@ -4164,24 +4251,24 @@ Module Compilers.
                   => Abs (fun x
                           => @reify d (f (@reflect s (Var x))))
              | type.list A as t
-               => fun x : expr t + list (value var A)
+               => fun x : _ * expr t + list (value var A)
                   => match x with
-                     | inl v => v
+                     | inl (_, v) => v
                      | inr v => reify_list (List.map (@reify A) v)
                      end
              | type.type_primitive type.Z as t
-               => fun x : Zdata * expr t + type.interp t
+               => fun x : _ * expr t + type.interp t
                   => match x with
                      | inl (Some r, v) => ident.Z.cast r @@ v
                      | inl (None, v) => v
                      | inr v => ident.primitive v @@ TT
                      end%core%expr
              | type.type_primitive _ as t
-               => fun x : expr t + type.interp t
+               => fun x : _ * expr t + type.interp t
                   => match x with
-                     | inl v => v
+                     | inl (_, v) => v
                      | inr v => ident.primitive v @@ TT
-                     end%expr
+                     end%core%expr
              end
         with reflect {t : type}
              : @expr var t -> value var t
@@ -4191,28 +4278,39 @@ Module Compilers.
                      => @reflect d (App f (@reify s x))
                 | type.prod A B as t
                   => fun v : expr t
-                     => let inr := @inr (expr t) (value_prestep (value var) t) in
-                        let inl := @inl (expr t) (value_prestep (value var) t) in
+                     => let inr := @inr (data t * expr t) (value_prestep (value var) t) in
+                        let inl := @inl (data t * expr t) (value_prestep (value var) t) in
                         match invert_Pair v with
                         | Some (a, b)
                           => inr (@reflect A a, @reflect B b)
                         | None
-                          => inl v
+                          => inl
+                               (match A, B return expr (A * B) -> data (A * B) * expr (A * B) with
+                                | type.Z, type.Z
+                                  => fun v
+                                     => match invert_Z_cast2 v with
+                                        | Some (r, v)
+                                          => (ZRange.type.option.Some (t:=type.Z*type.Z) r, v)
+                                        | None
+                                          => (ZRange.type.option.None, v)
+                                        end
+                                | _, _ => fun v => (ZRange.type.option.None, v)
+                                end v)
                         end
                 | type.list A as t
                   => fun v : expr t
-                     => let inr := @inr (expr t) (value_prestep (value var) t) in
-                        let inl := @inl (expr t) (value_prestep (value var) t) in
+                     => let inr := @inr (data t * expr t) (value_prestep (value var) t) in
+                        let inl := @inl (data t * expr t) (value_prestep (value var) t) in
                         match reflect_list v with
                         | Some ls
                           => inr (List.map (@reflect A) ls)
                         | None
-                          => inl v
+                          => inl (None, v)
                         end
                 | type.type_primitive type.Z as t
                   => fun v : expr t
-                     => let inr' := @inr (Zdata * expr t) (value_prestep (value var) t) in
-                        let inl' := @inl (Zdata * expr t) (value_prestep (value var) t) in
+                     => let inr' := @inr (data t * expr t) (value_prestep (value var) t) in
+                        let inl' := @inl (data t * expr t) (value_prestep (value var) t) in
                         match reflect_primitive v, invert_Z_cast v with
                         | Some v, _ => inr' v
                         | None, Some (r, v) => inl' (Some r, v)
@@ -4220,11 +4318,11 @@ Module Compilers.
                         end
                 | type.type_primitive _ as t
                   => fun v : expr t
-                     => let inr := @inr (expr t) (value_prestep (value var) t) in
-                        let inl := @inl (expr t) (value_prestep (value var) t) in
+                     => let inr := @inr (data t * expr t) (value_prestep (value var) t) in
+                        let inl := @inl (data t * expr t) (value_prestep (value var) t) in
                         match reflect_primitive v with
                         | Some v => inr v
-                        | None => inl v
+                        | None => inl (tt, v)
                         end
                 end.
       End reify.
@@ -4239,6 +4337,8 @@ Module Compilers.
              | TT => true
              | AppIdent _ _ (ident.fst _ _) args => @is_var_like _ args
              | AppIdent _ _ (ident.snd _ _) args => @is_var_like _ args
+             | AppIdent _ _ (ident.Z.cast _) args => @is_var_like _ args
+             | AppIdent _ _ (ident.Z.cast2 _) args => @is_var_like _ args
              | Pair A B a b => @is_var_like A a && @is_var_like B b
              | AppIdent _ _ _ _ => false
              | App _ _ _ _
@@ -4252,7 +4352,7 @@ Module Compilers.
              | type.arrow _ _
                => fun x f => f x
              | type.list T as t
-               => fun (x : expr t + list (value var T)) (f : expr t + list (value var T) -> value var tC)
+               => fun (x : data t * expr t + list (value var T)) (f : data t * expr t + list (value var T) -> value var tC)
                   => match x with
                      | inr ls
                        => list_rect
@@ -4267,7 +4367,7 @@ Module Compilers.
                      | inl e => f (inl e)
                      end
              | type.prod A B as t
-               => fun (x : expr t + value var A * value var B) (f : expr t + value var A * value var B -> value var tC)
+               => fun (x : data t * expr t + value var A * value var B) (f : data t * expr t + value var A * value var B -> value var tC)
                   => match x with
                      | inr (a, b)
                        => @interp_let_in
@@ -4276,11 +4376,12 @@ Module Compilers.
                              => @interp_let_in
                                   _ B b
                                   (fun b => f (inr (a, b))))
-                     | inl e => partial.expr.reflect (expr_let y := e in partial.expr.reify (f (inl (Var y))))%expr
+                     | inl (data, e) => partial.expr.reflect
+                                          (expr_let y := partial.expr.reify (t:=t) x in
+                                               partial.expr.reify (f (inl (data, Var y)%core)))%expr
                      end
-             | type.type_primitive type.Z as t
-               => fun (x : Zdata * expr t + type.interp t)
-                      (f : Zdata * expr t + type.interp t -> value var tC)
+             | type.type_primitive _ as t
+               => fun (x : data t * expr t + type.interp t) (f : data t * expr t + type.interp t -> value var tC)
                   => match x with
                      | inl (data, e)
                        => if is_var_like e
@@ -4288,74 +4389,73 @@ Module Compilers.
                           else partial.expr.reflect
                                  (expr_let y := (partial.expr.reify (t:=t) x) in
                                       partial.expr.reify (f (inl (data, Var y)%core)))%expr
-                     | inr v => f (inr v)
-                     end
-             | type.type_primitive _ as t
-               => fun (x : expr t + type.interp t) (f : expr t + type.interp t -> value var tC)
-                  => match x with
-                     | inl e
-                       => match invert_Var e with
-                          | Some _ => f x
-                          | None => partial.expr.reflect
-                                      (expr_let y := (partial.expr.reify (t:=t) x) in
-                                           partial.expr.reify (f (inl (Var y))))%expr
-                          end
                      | inr v => f (inr v) (* FIXME: do not substitute [S (big stuck term)] *)
                      end
+             end.
+
+        Let default_interp
+            {s d}
+          : ident s d -> value var s -> value var d
+          := match d return ident s d -> value var s -> value var d with
+             | type.arrow _ _
+               => fun idc args => expr.reflect (AppIdent idc (expr.reify args))
+             | _
+               => fun idc args
+                  => inl (ZRange.ident.option.interp idc (data_from_value var args),
+                          AppIdent idc (expr.reify args))
              end.
 
         (** do partial reduction on identifiers *)
         Definition interp {s d} (idc : ident s d) : value var (s -> d)
           := match idc in ident s d return value var (s -> d) with
              | ident.Let_In tx tC as idc
-               => fun (xf : expr (tx * (tx -> tC)) + value var tx * value var (tx -> tC))
+               => fun (xf : data (tx * (tx -> tC)) * expr (tx * (tx -> tC)) + value var tx * value var (tx -> tC))
                   => match xf with
                      | inr (x, f) => interp_let_in x f
                      | _ => expr.reflect (AppIdent idc (expr.reify (t:=tx * (tx -> tC)) xf))
                      end
              | ident.nil t
                => fun _ => inr (@nil (value var t))
-             | ident.primitive type.Z v
-               => fun _ => inr v
              | ident.primitive t v
                => fun _ => inr v
              | ident.cons t as idc
-               => fun (x_xs : expr (t * type.list t) + value var t * (expr (type.list t) + list (value var t)))
-                  => match x_xs return expr (type.list t) + list (value var t) with
+               => fun (x_xs : data (t * type.list t) * expr (t * type.list t) + value var t * (data (type.list t) * expr (type.list t) + list (value var t)))
+                  => match x_xs return data (type.list t) * expr (type.list t) + list (value var t) with
                      | inr (x, inr xs) => inr (cons x xs)
-                     | _ => expr.reflect (AppIdent idc (expr.reify (t:=t * type.list t) x_xs))
+                     | _
+                       => default_interp idc x_xs
                      end
              | ident.fst A B as idc
-               => fun x : expr (A * B) + value var A * value var B
+               => fun x : data (A * B) * expr (A * B) + value var A * value var B
                   => match x with
                      | inr x => fst x
-                     | _ => expr.reflect (AppIdent idc (expr.reify (t:=A*B) x))
+                     | _ => default_interp idc x
                      end
              | ident.snd A B as idc
-               => fun x : expr (A * B) + value var A * value var B
+               => fun x : data (A * B) * expr (A * B) + value var A * value var B
                   => match x with
                      | inr x => snd x
-                     | _ => expr.reflect (AppIdent idc (expr.reify (t:=A*B) x))
+                     | _ => default_interp idc x
                      end
              | ident.bool_rect T as idc
-               => fun (true_case_false_case_b : expr (T * T * type.bool) + (expr (T * T) + value var T * value var T) * (expr type.bool + bool))
+               => fun (true_case_false_case_b : data (T * T * type.bool) * expr (T * T * type.bool) + (data (T * T) * expr (T * T) + value var T * value var T) * (data type.bool * expr type.bool + bool))
                   => match true_case_false_case_b with
                      | inr (inr (true_case, false_case), inr b)
                        => @bool_rect (fun _ => value var T) true_case false_case b
-                     | _ => expr.reflect (AppIdent idc (expr.reify (t:=T*T*type.bool) true_case_false_case_b))
+                     | _ => default_interp idc true_case_false_case_b
                      end
              | ident.nat_rect P as idc
-               => fun (O_case_S_case_n : expr (P * (type.nat * P -> P) * type.nat) + (expr (P * (type.nat * P -> P)) + value var P * value var (type.nat * P -> P)) * (expr type.nat + nat))
+               => fun (O_case_S_case_n : _ * expr (P * (type.nat * P -> P) * type.nat) + (_ * expr (P * (type.nat * P -> P)) + value var P * value var (type.nat * P -> P)) * (_ * expr type.nat + nat))
                   => match O_case_S_case_n with
                      | inr (inr (O_case, S_case), inr n)
                        => @nat_rect (fun _ => value var P)
                                     O_case
                                     (fun n' rec => S_case (inr (inr n', rec)))
                                     n
-                     | _ => expr.reflect (AppIdent idc (expr.reify (t:=P * (type.nat * P -> P) * type.nat) O_case_S_case_n))
+                     | _ => default_interp idc O_case_S_case_n
                      end
              | ident.list_rect A P as idc
-               => fun (nil_case_cons_case_ls : expr (P * (A * type.list A * P -> P) * type.list A) + (expr (P * (A * type.list A * P -> P)) + value var P * value var (A * type.list A * P -> P)) * (expr (type.list A) + list (value var A)))
+               => fun (nil_case_cons_case_ls : _ * expr (P * (A * type.list A * P -> P) * type.list A) + (_ * expr (P * (A * type.list A * P -> P)) + value var P * value var (A * type.list A * P -> P)) * (_ * expr (type.list A) + list (value var A)))
                   => match nil_case_cons_case_ls with
                      | inr (inr (nil_case, cons_case), inr ls)
                        => @list_rect
@@ -4364,60 +4464,60 @@ Module Compilers.
                             nil_case
                             (fun x xs rec => cons_case (inr (inr (x, inr xs), rec)))
                             ls
-                     | _ => expr.reflect (AppIdent idc (expr.reify (t:=P * (A * type.list A * P -> P) * type.list A) nil_case_cons_case_ls))
+                     | _ => default_interp idc nil_case_cons_case_ls
                      end
              | ident.List.nth_default type.Z as idc
-               => fun (default_ls_idx : expr (type.Z * type.list type.Z * type.nat) + (expr (type.Z * type.list type.Z) + (_ * expr type.Z + type.interp type.Z) * (expr (type.list type.Z) + list (value var type.Z))) * (expr type.nat + nat))
+               => fun (default_ls_idx : _ * expr (type.Z * type.list type.Z * type.nat) + (_ * expr (type.Z * type.list type.Z) + (_ * expr type.Z + type.interp type.Z) * (_ * expr (type.list type.Z) + list (value var type.Z))) * (_ * expr type.nat + nat))
                   => match default_ls_idx with
                      | inr (inr (default, inr ls), inr idx)
                        => List.nth_default default ls idx
                      | inr (inr (inr default, ls), inr idx)
-                       => expr.reflect (AppIdent (ident.List.nth_default_concrete default idx) (expr.reify (t:=type.list type.Z) ls))
-                     | _ => expr.reflect (AppIdent idc (expr.reify (t:=type.Z * type.list type.Z * type.nat) default_ls_idx))
+                       => default_interp (ident.List.nth_default_concrete default idx) ls
+                     | _ => default_interp idc default_ls_idx
                      end
              | ident.List.nth_default (type.type_primitive A) as idc
-               => fun (default_ls_idx : expr (A * type.list A * type.nat) + (expr (A * type.list A) + (expr A + type.interp A) * (expr (type.list A) + list (value var A))) * (expr type.nat + nat))
+               => fun (default_ls_idx : _ * expr (A * type.list A * type.nat) + (_ * expr (A * type.list A) + (_ * expr A + type.interp A) * (_ * expr (type.list A) + list (value var A))) * (_ * expr type.nat + nat))
                   => match default_ls_idx with
                      | inr (inr (default, inr ls), inr idx)
                        => List.nth_default default ls idx
                      | inr (inr (inr default, ls), inr idx)
-                       => expr.reflect (AppIdent (ident.List.nth_default_concrete default idx) (expr.reify (t:=type.list A) ls))
-                     | _ => expr.reflect (AppIdent idc (expr.reify (t:=A * type.list A * type.nat) default_ls_idx))
+                       => default_interp (ident.List.nth_default_concrete default idx) ls
+                     | _ => default_interp idc default_ls_idx
                      end
              | ident.List.nth_default A as idc
-               => fun (default_ls_idx : expr (A * type.list A * type.nat) + (expr (A * type.list A) + value var A * (expr (type.list A) + list (value var A))) * (expr type.nat + nat))
+               => fun (default_ls_idx : _ * expr (A * type.list A * type.nat) + (_ * expr (A * type.list A) + value var A * (_ * expr (type.list A) + list (value var A))) * (_ * expr type.nat + nat))
                   => match default_ls_idx with
                      | inr (inr (default, inr ls), inr idx)
                        => List.nth_default default ls idx
-                     | _ => expr.reflect (AppIdent idc (expr.reify (t:=A * type.list A * type.nat) default_ls_idx))
+                     | _ => default_interp idc default_ls_idx
                      end
              | ident.List.nth_default_concrete A default idx as idc
-               => fun (ls : expr (type.list A) + list (value var A))
+               => fun (ls : _ * expr (type.list A) + list (value var A))
                   => match ls with
                      | inr ls
                        => List.nth_default (expr.reflect (t:=A) (AppIdent (ident.primitive default) TT)) ls idx
-                     | _ => expr.reflect (AppIdent idc (expr.reify (t:=type.list A) ls))
+                     | _ => default_interp idc ls
                      end
              | ident.Z_mul_split as idc
-               => fun (x_y_z :  (expr (type.Z * type.Z * type.Z) +
-                                 (expr (type.Z * type.Z) + (_ * expr type.Z + Z) * (_ * expr type.Z + Z)) * (_ * expr type.Z + Z))%type)
-                  => match x_y_z return (expr _ + (_ * expr _ + type.interp _) * (_ * expr _ + type.interp _)) with
+               => fun (x_y_z :  (_ * expr (type.Z * type.Z * type.Z) +
+                                 (_ * expr (type.Z * type.Z) + (_ * expr type.Z + Z) * (_ * expr type.Z + Z)) * (_ * expr type.Z + Z))%type)
+                  => match x_y_z return (_ * expr _ + (_ * expr _ + type.interp _) * (_ * expr _ + type.interp _)) with
                      | inr (inr (inr x, inr y), inr z) =>
                        let result := ident.interp idc (x, y, z) in
                        inr (inr (fst result), inr (snd result))
                      | inr (inr (inr x, y), z)
-                       => expr.reflect (AppIdent (ident.Z.mul_split_concrete x) (expr.reify (t:=type.Z*type.Z) (inr (y, z))))
-                     | _ => expr.reflect (AppIdent idc (expr.reify (t:=_*_*_) x_y_z))
+                       => default_interp (ident.Z.mul_split_concrete x) (inr (y, z))
+                     | _ => default_interp idc x_y_z
                      end
              | ident.Z_add_get_carry as idc
-               => fun (x_y_z :  (expr (type.Z * type.Z * type.Z) +
-                                 (expr (type.Z * type.Z) + (_ * expr type.Z + Z) * (_ * expr type.Z + Z)) * (_ * expr type.Z + Z))%type)
-                  => match x_y_z return (expr _ + (_ * expr _ + type.interp _) * (_ * expr _ + type.interp _)) with
+               => fun (x_y_z :  (_ * expr (type.Z * type.Z * type.Z) +
+                                 (_ * expr (type.Z * type.Z) + (_ * expr type.Z + Z) * (_ * expr type.Z + Z)) * (_ * expr type.Z + Z))%type)
+                  => match x_y_z return (_ * expr _ + (_ * expr _ + type.interp _) * (_ * expr _ + type.interp _)) with
                      | inr (inr (inr x, inr y), inr z) =>
                        let result := ident.interp idc (x, y, z) in
                        inr (inr (fst result), inr (snd result))
                      | inr (inr (inr x, y), z)
-                       => let default := expr.reflect (AppIdent (ident.Z.add_get_carry_concrete x) (expr.reify (t:=type.Z*type.Z) (inr (y, z)))) in
+                       => let default := default_interp (ident.Z.add_get_carry_concrete x) (inr (y, z)) in
                           match (y, z) with
                           | (inr xx, inl e)
                           | (inl e, inr xx)
@@ -4426,45 +4526,45 @@ Module Compilers.
                                else default
                           | _ => default
                           end
-                     | _ => expr.reflect (AppIdent idc (expr.reify (t:=_*_*_) x_y_z))
+                     | _ => default_interp idc x_y_z
                      end
              | ident.Z_add_with_get_carry as idc
-               => fun (x_y_z_a : (expr (_ * _ * _ * _) +
-                                  (expr (_ * _ * _) +
-                                   (expr (_ * _) + (_ * expr _ + type.interp _) * (_ * expr _ + type.interp _)) *
+               => fun (x_y_z_a : (_ * expr (_ * _ * _ * _) +
+                                  (_ * expr (_ * _ * _) +
+                                   (_ * expr (_ * _) + (_ * expr _ + type.interp _) * (_ * expr _ + type.interp _)) *
                                    (_ * expr _ + type.interp _)) * (_ * expr _ + type.interp _))%type)
-                  => match x_y_z_a return (expr _ + (_ * expr _ + type.interp _) * (_ * expr _ + type.interp _)) with
+                  => match x_y_z_a return (_ * expr _ + (_ * expr _ + type.interp _) * (_ * expr _ + type.interp _)) with
                      | inr (inr (inr (inr x, inr y), inr z), inr a) =>
                        let result := ident.interp idc (x, y, z, a) in
                        inr (inr (fst result), inr (snd result))
                      | inr (inr (inr (inr x, y), z), a)
-                        => expr.reflect (AppIdent (ident.Z.add_with_get_carry_concrete x) (expr.reify (t:=type.Z*type.Z*type.Z) (inr (inr (y, z), a))))
-                     | _ => expr.reflect (AppIdent idc (expr.reify (t:=_*_*_*_) x_y_z_a))
+                        => default_interp (ident.Z.add_with_get_carry_concrete x) (inr (inr (y, z), a))
+                     | _ => default_interp idc x_y_z_a
                      end
              | ident.Z_sub_get_borrow as idc
-               => fun (x_y_z :  (expr (type.Z * type.Z * type.Z) +
-                                 (expr (type.Z * type.Z) + (_ * expr type.Z + Z) * (_ * expr type.Z + Z)) * (_ * expr type.Z + Z))%type)
-                  => match x_y_z return (expr _ + (_ * expr _ + type.interp _) * (_ * expr _ + type.interp _)) with
+               => fun (x_y_z :  (_ * expr (type.Z * type.Z * type.Z) +
+                                 (_ * expr (type.Z * type.Z) + (_ * expr type.Z + Z) * (_ * expr type.Z + Z)) * (_ * expr type.Z + Z))%type)
+                  => match x_y_z return (_ * expr _ + (_ * expr _ + type.interp _) * (_ * expr _ + type.interp _)) with
                      | inr (inr (inr x, inr y), inr z) =>
                        let result := ident.interp idc (x, y, z) in
                        inr (inr (fst result), inr (snd result))
                      | inr (inr (inr x, y), z)
-                       => expr.reflect (AppIdent (ident.Z.sub_get_borrow_concrete x) (expr.reify (t:=type.Z*type.Z) (inr (y, z))))
-                     | _ => expr.reflect (AppIdent idc (expr.reify (t:=_*_*_) x_y_z))
+                       => default_interp (ident.Z.sub_get_borrow_concrete x) (inr (y, z))
+                     | _ => default_interp idc x_y_z
                      end
              | ident.Z_mul_split_concrete _ as idc
              | ident.Z.sub_get_borrow_concrete _ as idc
-               => fun (x_y : expr (_ * _) + (_ * expr _ + type.interp _) * (_ * expr _ + type.interp _))
-                  => match x_y return (expr _ + (_ * expr _ + type.interp _) * (_ * expr _ + type.interp _)) with
+               => fun (x_y : _ * expr (_ * _) + (_ * expr _ + type.interp _) * (_ * expr _ + type.interp _))
+                  => match x_y return (_ * expr _ + (_ * expr _ + type.interp _) * (_ * expr _ + type.interp _)) with
                      | inr (inr x, inr y) =>
                        let result := ident.interp idc (x, y) in
                        inr (inr (fst result), inr (snd result))
-                     | _ => expr.reflect (AppIdent idc (expr.reify (t:=_*_) x_y))
+                     | _ => default_interp idc x_y
                      end
              | ident.Z.add_get_carry_concrete _ as idc
-               => fun (x_y : expr (_ * _) + (_ * expr _ + type.interp _) * (_ * expr _ + type.interp _))
-                  => let default := expr.reflect (AppIdent idc (expr.reify (t:=_*_) x_y)) in
-                     match x_y return (expr _ + (_ * expr _ + type.interp _) * (_ * expr _ + type.interp _)) with
+               => fun (x_y : _ * expr (_ * _) + (_ * expr _ + type.interp _) * (_ * expr _ + type.interp _))
+                  => let default := default_interp idc x_y in
+                     match x_y return (_ * expr _ + (_ * expr _ + type.interp _) * (_ * expr _ + type.interp _)) with
                      | inr (inr x, inr y) =>
                        let result := ident.interp idc (x, y) in
                        inr (inr (fst result), inr (snd result))
@@ -4476,26 +4576,26 @@ Module Compilers.
                      | _ => default
                      end
              | ident.Z.add_with_get_carry_concrete _ as idc
-               => fun (x_y_z :  (expr (type.Z * type.Z * type.Z) +
-                                 (expr (type.Z * type.Z) + (_ * expr type.Z + Z) * (_ * expr type.Z + Z)) * (_ * expr type.Z + Z))%type)
-                  => match x_y_z return (expr _ + (_ * expr _ + type.interp _) * (_ * expr _ + type.interp _)) with
+               => fun (x_y_z :  (_ * expr (type.Z * type.Z * type.Z) +
+                                 (_ * expr (type.Z * type.Z) + (_ * expr type.Z + Z) * (_ * expr type.Z + Z)) * (_ * expr type.Z + Z))%type)
+                  => match x_y_z return (_ * expr _ + (_ * expr _ + type.interp _) * (_ * expr _ + type.interp _)) with
                      | inr (inr (inr x, inr y), inr z) =>
                        let result := ident.interp idc (x, y, z) in
                        inr (inr (fst result), inr (snd result))
-                     | _ => expr.reflect (AppIdent idc (expr.reify (t:=_*_*_) x_y_z))
+                     | _ => default_interp idc x_y_z
                      end
              | ident.pred as idc
              | ident.Nat_succ as idc
-               => fun x : expr _ + type.interp _
-                  => match x return expr _ + type.interp _ with
-                     | inr x => inr (ident.interp idc x)
-                     | inl x => expr.reflect (AppIdent idc x)
-                     end
-             | ident.Z_of_nat as idc
-               => fun x : expr _ + type.interp _
+               => fun x : _ * expr _ + type.interp _
                   => match x return _ * expr _ + type.interp _ with
                      | inr x => inr (ident.interp idc x)
-                     | inl x => expr.reflect (AppIdent idc x)
+                     | _ => default_interp idc x
+                     end
+             | ident.Z_of_nat as idc
+               => fun x : _ * expr _ + type.interp _
+                  => match x return _ * expr _ + type.interp _ with
+                     | inr x => inr (ident.interp idc x)
+                     | _ => default_interp idc x
                      end
              | ident.Z_opp as idc
                => fun x : _ * expr _ + type.interp _
@@ -4522,36 +4622,36 @@ Module Compilers.
              | ident.Z_eqb as idc
              | ident.Z_leb as idc
              | ident.Z_pow as idc
-               => fun (x_y : expr (_ * _) + (_ + type.interp _) * (_ + type.interp _))
+               => fun (x_y : data (_ * _) * expr (_ * _) + (_ + type.interp _) * (_ + type.interp _))
                   => match x_y return _ + type.interp _ with
                      | inr (inr x, inr y) => inr (ident.interp idc (x, y))
-                     | _ => expr.reflect (AppIdent idc (expr.reify (t:=_*_) x_y))
+                     | _ => default_interp idc x_y
                      end
              | ident.Z_div as idc
-               => fun (x_y : expr (_ * _) + (_ * expr _ + type.interp _) * (_ * expr _ + type.interp _))
-                  => let default := expr.reflect (AppIdent idc (expr.reify (t:=_*_) x_y)) in
+               => fun (x_y : _ * expr (_ * _) + (_ * expr _ + type.interp _) * (_ * expr _ + type.interp _))
+                  => let default := default_interp idc x_y in
                      match x_y return _ * expr _ + type.interp _ with
                      | inr (inr x, inr y) => inr (ident.interp idc (x, y))
                      | inr (x, inr y)
                        => if Z.eqb y (2^Z.log2 y)
-                          then expr.reflect (AppIdent (ident.Z.shiftr (Z.log2 y)) (expr.reify (t:=type.Z) x))
+                          then default_interp (ident.Z.shiftr (Z.log2 y)) x
                           else default
                      | _ => default
                      end
              | ident.Z_modulo as idc
-               => fun (x_y : expr (_ * _) + (_ * expr _ + type.interp _) * (_ * expr _ + type.interp _))
-                  => let default := expr.reflect (AppIdent idc (expr.reify (t:=_*_) x_y)) in
+               => fun (x_y : _ * expr (_ * _) + (_ * expr _ + type.interp _) * (_ * expr _ + type.interp _))
+                  => let default := default_interp idc x_y in
                      match x_y return _ * expr _ + type.interp _ with
                      | inr (inr x, inr y) => inr (ident.interp idc (x, y))
                      | inr (x, inr y)
                        => if Z.eqb y (2^Z.log2 y)
-                          then expr.reflect (AppIdent (ident.Z.land (y-1)) (expr.reify (t:=type.Z) x))
+                          then default_interp (ident.Z.land (y-1)) x
                           else default
                      | _ => default
                      end
              | ident.Z_mul as idc
-               => fun (x_y : expr (_ * _) + (_ * expr _ + type.interp _) * (_ * expr _ + type.interp _))
-                  => let default := expr.reflect (AppIdent idc (expr.reify (t:=_*_) x_y)) in
+               => fun (x_y : _ * expr (_ * _) + (_ * expr _ + type.interp _) * (_ * expr _ + type.interp _))
+                  => let default := default_interp idc x_y in
                      match x_y return _ * expr _ + type.interp _ with
                      | inr (inr x, inr y) => inr (ident.interp idc (x, y))
                      | inr (inr x, inl (data, e) as y)
@@ -4574,7 +4674,7 @@ Module Compilers.
                      | inl _ => default
                      end
              | ident.Z_add as idc
-               => fun (x_y : expr (_ * _) + (_ * expr _ + type.interp _) * (_ * expr _ + type.interp _))
+               => fun (x_y : _ * expr (_ * _) + (_ * expr _ + type.interp _) * (_ * expr _ + type.interp _))
                   => let default0 := AppIdent idc (expr.reify (t:=_*_) x_y) in
                      let default := expr.reflect default0 in
                      match x_y return _ * expr _ + type.interp _ with
@@ -4608,7 +4708,7 @@ Module Compilers.
                      | inl _ => default
                      end
              | ident.Z_sub as idc
-               => fun (x_y : expr (_ * _) + (_ * expr _ + type.interp _) * (_ * expr _ + type.interp _))
+               => fun (x_y : _ * expr (_ * _) + (_ * expr _ + type.interp _) * (_ * expr _ + type.interp _))
                   => let default0 := AppIdent idc (expr.reify (t:=_*_) x_y) in
                      let default := expr.reflect default0 in
                      match x_y return _ * expr _ + type.interp _ with
@@ -4641,16 +4741,34 @@ Module Compilers.
                      end
              | ident.Z_zselect as idc
              | ident.Z_add_modulo as idc
-               => fun (x_y_z :  (expr (_ * _ * _) +
-                                 (expr (_ * _) + (_ * expr _ + type.interp _) * (_ * expr _ + type.interp _)) * (_ * expr _ + type.interp _))%type)
+               => fun (x_y_z :  (_ * expr (_ * _ * _) +
+                                 (_ * expr (_ * _) + (_ * expr _ + type.interp _) * (_ * expr _ + type.interp _)) * (_ * expr _ + type.interp _))%type)
                   => match x_y_z return _ * expr _ + type.interp _ with
                      | inr (inr (inr x, inr y), inr z) => inr (ident.interp idc (x, y, z))
-                     | _ => expr.reflect (AppIdent idc (expr.reify (t:=_*_*_) x_y_z))
+                     | _ => default_interp idc x_y_z
                      end
              | ident.Z_cast r as idc
                => fun (x : _ * expr _ + type.interp _)
                   => match x with
                      | inr x => inr (ident.interp idc x)
+                     | inl (data, e)
+                       => inl (ZRange.ident.option.interp idc data, e)
+                     end
+             | ident.Z_cast2 (r1, r2) as idc
+               => fun (x : _ * expr _ + (_ * expr _ + type.interp _) * (_ * expr _ + type.interp _))
+                  => match x with
+                     | inr (inr a, inr b)
+                       => inr (inr (ident.interp (ident.Z.cast r1) a),
+                               inr (ident.interp (ident.Z.cast r2) b))
+                     | inr (inr a, inl (r2', b))
+                       => inr (inr (ident.interp (ident.Z.cast r1) a),
+                               inl (ZRange.ident.option.interp (ident.Z.cast r2) r2', b))
+                     | inr (inl (r1', a), inr b)
+                       => inr (inl (ZRange.ident.option.interp (ident.Z.cast r1) r1', a),
+                               inr (ident.interp (ident.Z.cast r2) b))
+                     | inr (inl (r1', a), inl (r2', b))
+                       => inr (inl (ZRange.ident.option.interp (ident.Z.cast r1) r1', a),
+                               inl (ZRange.ident.option.interp (ident.Z.cast r2) r2', b))
                      | inl (data, e)
                        => inl (ZRange.ident.option.interp idc data, e)
                      end
@@ -4712,37 +4830,74 @@ Module Compilers.
              | type.type_primitive t => fun _ => id
              | type.prod A B
                => fun '((ra, rb) : ZRange.type.option.interp A * ZRange.type.option.interp B)
-                      (e : expr _ + partial.value var A * partial.value var B)
+                      (e : _ * expr _ + partial.value var A * partial.value var B)
                   => match e with
                      | inr (a, b)
                        => inr (@extend_with_obounds A ra a,
                                @extend_with_obounds B rb b)
-                     | inl e
+                     | inl ((dataa, datab), e)
                        => if partial.ident.is_var_like e
                           then inr (@extend_with_obounds A ra (partial.expr.reflect (AppIdent ident.fst e)),
                                     @extend_with_obounds B rb (partial.expr.reflect (AppIdent ident.snd e)))
-                          else inl e
+                          else inl
+                                 (match A, B return ZRange.type.option.interp A  -> ZRange.type.option.interp B -> data A -> data B -> expr (A * B) -> data (A * B) * expr (A * B) with
+                                  | type.Z, type.Z
+                                    => fun ra rb da db e
+                                       => let da'
+                                              := match ra with
+                                                 | Some ra
+                                                   => ZRange.ident.option.interp
+                                                        (ident.Z.cast ra) da
+                                                 | None => da
+                                                 end in
+                                          let db'
+                                              := match rb with
+                                                 | Some rb
+                                                   => ZRange.ident.option.interp
+                                                        (ident.Z.cast rb) db
+                                                 | None => db
+                                                 end in
+                                          ((da', db'), e)
+                                  | _, _
+                                    => fun _ _ da db e => ((da, db), e)
+                                  end ra rb dataa datab e)
                      end
              | type.arrow s d => fun _ => id
              | type.list A
-               => fun (ls : Datatypes.list (ZRange.type.option.interp A))
-                      (e : expr _ + list (partial.value var A))
-                  => match e with
-                     | inl e
-                       => match A return (ZRange.type.option.interp A -> partial.value var A -> partial.value var A)
-                                         -> Datatypes.list (ZRange.type.option.interp A)
-                                         -> expr (type.list A)
-                                         -> partial.value var (type.list A)
-                          with
-                          | type.type_primitive A
-                            => fun extend_with_obounds ls e
-                               => inr (extend_list_expr_with_obounds
-                                         extend_with_obounds 0 ls e)
-                          | A'
-                            => fun _ _ e => inl e
-                          end (@extend_with_obounds A) ls e
-                     | inr e => inr (extend_concrete_list_with_obounds
-                                       (@extend_with_obounds A) ls e)
+               => fun (ls : option (Datatypes.list (ZRange.type.option.interp A)))
+                      (e : data _ * expr _ + list (partial.value var A))
+                  => match ls with
+                     | None => e
+                     | Some ls
+                       =>
+                       match e with
+                       | inl (data, e)
+                         => match A return (ZRange.type.option.interp A -> partial.value var A -> partial.value var A)
+                                           -> Datatypes.list (ZRange.type.option.interp A)
+                                           -> option (Datatypes.list (ZRange.type.option.interp A))
+                                           -> expr (type.list A)
+                                           -> partial.value var (type.list A)
+                            with
+                            | type.type_primitive A
+                              => fun extend_with_obounds ls data e
+                                 => match data with
+                                    | Some data
+                                      => inr
+                                           (extend_concrete_list_with_obounds
+                                              extend_with_obounds ls
+                                              (extend_list_expr_with_obounds
+                                                 extend_with_obounds 0 data e))
+                                    | None
+                                      => inr (extend_list_expr_with_obounds
+                                                extend_with_obounds 0 ls e)
+                                    end
+                            | A'
+                                (* N.B. We clobber the existing bounds here, rather than fusing them *)
+                              => fun _ ls data e => inl (Some ls, e)
+                            end (@extend_with_obounds A) ls data e
+                       | inr e => inr (extend_concrete_list_with_obounds
+                                         (@extend_with_obounds A) ls e)
+                       end
                      end
              end.
         Definition extend_with_bounds {t}
@@ -4761,10 +4916,10 @@ Module Compilers.
              | ident.Z_cast range => fun _ => Some range
              | ident.primitive type.Z v
                => fun _ => Some r[v~>v]%zrange
-             | ident.nil _ => fun _ => nil
+             | ident.nil _ => fun _ => Some nil
              | ident.cons t
-               => fun '((x, xs) : ZRange.type.option.interp t * list (ZRange.type.option.interp t))
-                  => cons x xs
+               => fun '((x, xs) : ZRange.type.option.interp t * option (list (ZRange.type.option.interp t)))
+                  => option_map (cons x) xs
              | _ => fun _ => ZRange.type.option.None
              end.
       End ident.
@@ -4798,7 +4953,10 @@ Module Compilers.
   Section partial_reduce.
     Context {var : type -> Type}.
 
-    Fixpoint partial_reduce' {t} (e : @expr (partial.value var) t)
+    Definition partial_reduce'_step
+               (partial_reduce' : forall {t} (e : @expr (partial.value var) t),
+                   partial.value var t)
+               {t} (e : @expr (partial.value var) t)
       : partial.value var t
       := match e in expr.expr t return partial.value var t with
          | Var t v => v
@@ -4808,6 +4966,9 @@ Module Compilers.
          | App s d f x => @partial_reduce' _ f (@partial_reduce' _ x)
          | Abs s d f => fun x => @partial_reduce' d (f x)
          end.
+    Fixpoint partial_reduce' {t} (e : @expr (partial.value var) t)
+      : partial.value var t
+      := @partial_reduce'_step (@partial_reduce') t e.
 
     Definition partial_reduce {t} (e : @expr (partial.value var) t) : @expr var t
       := partial.expr.reify (@partial_reduce' t e).
@@ -4839,6 +5000,12 @@ Module Compilers.
                => match relax_zrange range with
                   | Some r => AppIdent (ident.Z.cast r)
                   | None => id
+                  end
+             | ident.Z_cast2 (r1, r2)
+               => match relax_zrange r1, relax_zrange r2 with
+                  | Some r1, Some r2
+                    => AppIdent (ident.Z.cast2 (r1, r2))
+                  | Some _, None | None, Some _ | None, None => id
                   end
              | idc => AppIdent idc
              end.
@@ -6293,7 +6460,7 @@ Ltac solve_rone := solve_rop rone_correct.
 
 Module PrintingNotations.
   Export ident.
-  Global Set Printing Width 100000.
+  (*Global Set Printing Width 100000.*)
   Open Scope zrange_scope.
   Notation "'uint256'"
     := (r[0 ~> 115792089237316195423570985008687907853269984665640564039457584007913129639935]%zrange) : zrange_scope.
@@ -6303,6 +6470,8 @@ Module PrintingNotations.
     := (r[0 ~> 18446744073709551615]) : zrange_scope.
   Notation "'uint32'"
     := (r[0 ~> 4294967295]) : zrange_scope.
+  Notation "'bool'"
+    := (r[0 ~> 1]%zrange) : zrange_scope.
   Notation "ls [[ n ]]"
     := ((List.nth_default_concrete _ n @@ ls)%expr)
          (at level 30, format "ls [[ n ]]") : expr_scope.
@@ -6310,12 +6479,16 @@ Module PrintingNotations.
     := ((ident.Z.cast range @@ (List.nth_default_concrete _ n @@ ls))%expr)
          (format "( range )( ls [[ n ]] )") : expr_scope.
   (*Notation "( range )( v )" := (ident.Z.cast range @@ v)%expr : expr_scope.*)
+  Notation "x *₂₅₆ y"
+    := (ident.Z.cast uint256 @@ (ident.Z.mul @@ (x, y)))%expr (at level 40) : expr_scope.
   Notation "x *₁₂₈ y"
     := (ident.Z.cast uint128 @@ (ident.Z.mul @@ (x, y)))%expr (at level 40) : expr_scope.
   Notation "x *₆₄ y"
     := (ident.Z.cast uint64 @@ (ident.Z.mul @@ (x, y)))%expr (at level 40) : expr_scope.
   Notation "x *₃₂ y"
     := (ident.Z.cast uint32 @@ (ident.Z.mul @@ (x, y)))%expr (at level 40) : expr_scope.
+  Notation "x +₂₅₆ y"
+    := (ident.Z.cast uint256 @@ (ident.Z.add @@ (x, y)))%expr (at level 50) : expr_scope.
   Notation "x +₁₂₈ y"
     := (ident.Z.cast uint128 @@ (ident.Z.add @@ (x, y)))%expr (at level 50) : expr_scope.
   Notation "x +₆₄ y"
@@ -6341,8 +6514,17 @@ Module PrintingNotations.
     := ((ident.Z.cast out_t @@ (ident.Z.land mask @@ v))%expr)
          (format "( ( out_t )( v )  &  mask )")
        : expr_scope.
-  Notation "v ₁" := (ident.fst @@ v)%expr (at level 10, format "v ₁") : expr_scope.
-  Notation "v ₂" := (ident.snd @@ v)%expr (at level 10, format "v ₂") : expr_scope.
+
+  Notation "x" := (ident.Z.cast _ @@ Var x)%expr (only printing, at level 9) : expr_scope.
+  Notation "x" := (ident.Z.cast2 _ @@ Var x)%expr (only printing, at level 9) : expr_scope.
+  Notation "v ₁" := (ident.fst @@ Var v)%expr (at level 10, format "v ₁") : expr_scope.
+  Notation "v ₂" := (ident.snd @@ Var v)%expr (at level 10, format "v ₂") : expr_scope.
+  Notation "v ₁" := (ident.Z.cast _ @@ (ident.fst @@ Var v))%expr (at level 10, format "v ₁") : expr_scope.
+  Notation "v ₂" := (ident.Z.cast _ @@ (ident.snd @@ Var v))%expr (at level 10, format "v ₂") : expr_scope.
+  Notation "v ₁" := (ident.Z.cast _ @@ (ident.fst @@ (ident.Z.cast2 _ @@ Var v)))%expr (at level 10, format "v ₁") : expr_scope.
+  Notation "v ₂" := (ident.Z.cast _ @@ (ident.snd @@ (ident.Z.cast2 _ @@ Var v)))%expr (at level 10, format "v ₂") : expr_scope.
+
+
   (*Notation "ls [[ n ]]" := (List.nth_default_concrete _ n @@ ls)%expr : expr_scope.
   Notation "( range )( v )" := (ident.Z.cast range @@ v)%expr : expr_scope.
   Notation "x *₁₂₈ y"
@@ -6408,13 +6590,12 @@ Module PrintingNotations.
   (* TODO: come up with a better notation for arithmetic with carries
   that still distinguishes it from arithmetic without carries? *)
   Local Notation "'TwoPow256'" := 115792089237316195423570985008687907853269984665640564039457584007913129639936 (only parsing).
-  (*Notation "'ADD_256'" := (add_get_carry_concrete _ _ uint256 _ TwoPow256) : nexpr_scope.
-  Notation "'ADD_128'" := (add_get_carry_concrete _ _ uint128 _ TwoPow256) : nexpr_scope.
-  Notation "'ADDC_256'" := (add_with_get_carry_concrete _ _ _ uint256 _ TwoPow256) : nexpr_scope.
-  Notation "'SUB_256'" := (sub_get_borrow_concrete _ _ uint256 _ TwoPow256) : nexpr_scope.
-  Notation "'ADDM'" := (add_modulo _ _ _ uint256) : nexpr_scope.
-  Notation "'SELC'" := (zselect _ _ _ uint256) : nexpr_scope.
-  Notation "'MUL_256'" := (mul uint128 uint128 uint256) : nexpr_scope.*)
+  Notation "'ADD_256' ( x ,  y )" := (ident.Z.cast2 (uint256, bool)%core @@ (ident.Z.add_get_carry_concrete TwoPow256 @@ (x, y)))%expr : expr_scope.
+  Notation "'ADD_128' ( x ,  y )" := (ident.Z.cast2 (uint128, bool)%core @@ (ident.Z.add_get_carry_concrete TwoPow256 @@ (x, y)))%expr : expr_scope.
+  Notation "'ADDC_256' ( x ,  y ,  z )" := (ident.Z.cast2 (uint256, bool)%core @@ (ident.Z.add_with_get_carry_concrete TwoPow256 @@ (x, y, z)))%expr : expr_scope.
+  Notation "'SUB_256' ( x ,  y )" := (ident.Z.cast2 (uint256, bool)%core @@ (ident.Z.sub_get_borrow_concrete TwoPow256 @@ (x, y)))%expr : expr_scope.
+  Notation "'ADDM' ( x ,  y ,  z )" := (ident.Z.cast uint256 @@ (ident.Z.add_modulo @@ (x, y, z)))%expr : expr_scope.
+  Notation "'SELC' ( x ,  y ,  z )" := (ident.Z.cast uint256 @@ (ident.Z.zselect @@ (x, y, z)))%expr : expr_scope.
 End PrintingNotations.
 
 (*
@@ -7003,6 +7184,9 @@ Module MontgomeryReduction.
                       = montred' N R N' w w_half n lo_hi)
          As montred_gen_correct.
   Proof. Time cache_reify (). exact admit. (* correctness of initial parts of the pipeline *) Time Qed.
+  Module Export ReifyHints.
+    Global Hint Extern 1 (_ = montred' _ _ _ _ _ _ _) => simple apply montred_gen_correct : reify_gen_cache.
+  End ReifyHints.
 
   Section rmontred.
     Context (N R N' : Z)
@@ -7012,7 +7196,7 @@ Module MontgomeryReduction.
     Let bound := r[0 ~> (2^machine_wordsize - 1)%Z]%zrange.
 
     Definition relax_zrange_of_machine_wordsize
-      := relax_zrange_gen [machine_wordsize / 2; machine_wordsize; 2 * machine_wordsize; 4 * machine_wordsize]%Z.
+      := relax_zrange_gen [1; machine_wordsize / 2; machine_wordsize; 2 * machine_wordsize; 4 * machine_wordsize]%Z.
     Local Arguments relax_zrange_of_machine_wordsize / .
 
     Let rw := rweight machine_wordsize.
@@ -7033,7 +7217,7 @@ Module MontgomeryReduction.
               else res.
 
     Notation BoundsPipeline_correct in_bounds out_bounds op
-      := (fun (rop : Expr (type.reify_type_of op%function)) rv Hrop
+      := (fun rv (rop : Expr (type.reify_type_of op%function)) E Hrop HE
           => @Pipeline.BoundsPipeline_correct_trans
                true (* DCE *)
                relax_zrange
@@ -7043,7 +7227,7 @@ Module MontgomeryReduction.
                in_bounds
                out_bounds
                op
-               Hrop rv)
+               Hrop rv E HE)
            (only parsing).
 
     Definition rmontred_correct
@@ -7052,9 +7236,9 @@ Module MontgomeryReduction.
            bound
            (montred' N R N' (Interp rw) (Interp rw_half) 2).
 
-    Notation type_of_strip_2arrow := ((fun s s' (d : Prop) (_ : s -> s' -> d) => d) _ _ _).
+    Notation type_of_strip_5arrow := ((fun (d : Prop) (_ : forall A B C D E, d) => d) _).
     Definition rmontred_correctT rv : Prop
-      := exists rop, type_of_strip_2arrow (@rmontred_correct rop rv).
+      := type_of_strip_5arrow (@rmontred_correct rv).
   End rmontred.
 End MontgomeryReduction.
 
@@ -7071,217 +7255,166 @@ Module Montgomery256.
   Derive montred256
          SuchThat (MontgomeryReduction.rmontred_correctT N R N' machine_wordsize montred256)
          As montred256_correct.
-  Proof.
-    eexists; eapply MontgomeryReduction.rmontred_correct with (machine_wordsize:=machine_wordsize).
-    Time do_inline_cache_reify ltac:(fun _ => idtac).
-    cbv [Pipeline.BoundsPipeline].
-    set (k := PartialReduce _).
-    cbv [CheckedPartialReduceWithBounds1].
-    Time set (k' := PartialReduceWithBounds1 _ _).
-    Time lazy in k'.
-    Print fold_left.
-    Time lazy; reflexivity.
-    Time lazy -[Let_In k'].
-  | (* Doing [lazy] is twice as slow as doing [lazy -[Let_In]; lazy].
-  This is because the bounds pipeline does [dlet E : Expr := (reduced
-  thing) in let b := extract_bounds E in ...].  If we allow [lazy] to
-  unfold [Let_In] before it fully reduces the function (function,
-  because [Expr := forall var, @expr var]), then there is no sharing
-  between the partial reduction in bounds extraction and the partial
-  reduction in the return value.  So we force [lazy] to fully reduce
-  the argument first, and only then permit [lazy] to inline it.  This
-  is slightly slower than doing bounds analysis in a non-PHOAS
-  representation; we spend about 3%-5% of the overall time doing
-  bounds extraction, and fully reducing the bounds extraction
-  expression before plugging in arguments costs a bit more.  However,
-  it's still reasonably fast, and the code is much simpler when
-  [Interp] always succeeds rather than returning [option]. *)
-  lazy -[Let_In]; lazy; reflexivity ].
-
-    Time solve_rmontred_nocache machine_wordsize.
-    eapply MontgomeryReduction.rmontred_correct.
-    cbv [MontgomeryReduction.rmontred].
-    cbv [Pipeline.BoundsPipeline].
-    cbv [CheckedPartialReduceWithBounds1].
-    set (k := PartialReduceWithBounds1 _ _).
-    Timeout 10 Time lazy in k.
-    Time solve_rmontred(). Time Qed.
+  Proof. Time solve_rmontred machine_wordsize. Time Qed.
 
   Import PrintingNotations.
-  Open Scope nexpr_scope.
+  Open Scope expr_scope.
   Set Printing Width 100000.
+
   Print montred256.
-  (*
-    expr_let 3 := (uint128)(fst @@ x_1 >> 128) in
-    expr_let 4 := ((uint128)fst @@ x_1 & 340282366920938463463374607431768211455) in
-    expr_let 5 := MUL_256 @@ (x_3, (79228162514264337593543950337)) in
-    expr_let 7 := ((uint128)x_5 & 340282366920938463463374607431768211455) in
-    expr_let 8 := MUL_256 @@ (x_4, (340282366841710300986003757985643364352)) in
-    expr_let 10 := ((uint128)x_8 & 340282366920938463463374607431768211455) in
-    expr_let 11 := (uint128)(x_10 << 128) in
-    expr_let 12 := (uint128)(x_7 << 128) in
-    expr_let 17 := MUL_256 @@ (x_4, (79228162514264337593543950337)) in
-    expr_let 18 := ADD_128 @@ (x_11, x_12) in
-    expr_let 19 := ADD_256 @@ (x_17, fst @@ x_18) in
-    expr_let 43 := (uint128)(fst @@ x_19 >> 128) in
-    expr_let 44 := ((uint128)fst @@ x_19 & 340282366920938463463374607431768211455) in
-    expr_let 45 := MUL_256 @@ (x_43, (79228162514264337593543950335)) in
-    expr_let 46 := (uint128)(x_45 >> 128) in
-    expr_let 47 := ((uint128)x_45 & 340282366920938463463374607431768211455) in
-    expr_let 48 := MUL_256 @@ (x_44, (340282366841710300967557013911933812736)) in
-    expr_let 49 := (uint128)(x_48 >> 128) in
-    expr_let 50 := ((uint128)x_48 & 340282366920938463463374607431768211455) in
-    expr_let 51 := (uint128)(x_50 << 128) in
-    expr_let 52 := (uint128)(x_47 << 128) in
-    expr_let 57 := MUL_256 @@ (x_44, (79228162514264337593543950335)) in
-    expr_let 58 := ADD_128 @@ (x_51, x_52) in
-    expr_let 59 := ADD_256 @@ (x_57, fst @@ x_58) in
-    expr_let 60 := snd @@ x_59 +₁₂₈ snd @@ x_58 in
-    expr_let 67 := MUL_256 @@ (x_43, (340282366841710300967557013911933812736)) in
-    expr_let 69 := ADD_256 @@ (x_46, x_67) in
-    expr_let 70 := ADD_256 @@ (x_49, fst @@ x_69) in
-    expr_let 80 := ADD_256 @@ (x_60, fst @@ x_70) in
-    expr_let 83 := ADD_256 @@ (fst @@ x_1, fst @@ x_59) in
-    expr_let 84 := ADDC_256 @@ (snd @@ x_83, snd @@ x_1, fst @@ x_80) in
-    expr_let 85 := SELC @@ (snd @@ x_84, (0), (115792089210356248762697446949407573530086143415290314195533631308867097853951)) in
-    expr_let 86 := fst @@ (SUB_256 @@ (fst @@ x_84, x_85)) in
-    ADDM @@ (x_86, (0), (115792089210356248762697446949407573530086143415290314195533631308867097853951))
-         : expr uint256
-   *)
+  (*montred256 = fun var : type -> Type => λ v : var (type.type_primitive type.Z * type.type_primitive type.Z)%ctype,
+             expr_let v0 := (uint128)(v₁ >> 128) in
+             expr_let v1 := ((uint128)(v₁) & 340282366920938463463374607431768211455) in
+             expr_let v2 := ((uint128)(79228162514264337593543950337 *₂₅₆ v0) & 340282366920938463463374607431768211455) in
+             expr_let v3 := ((uint128)(340282366841710300986003757985643364352 *₂₅₆ v1) & 340282366920938463463374607431768211455) in
+             expr_let v4 := ADD_256 ((uint256)(v3 << 128), (uint256)(v2 << 128)) in
+             expr_let v5 := ADD_256 (79228162514264337593543950337 *₂₅₆ v1, v4₁) in
+             expr_let v6 := (uint128)(v5₁ >> 128) in
+             expr_let v7 := ((uint128)(v5₁) & 340282366920938463463374607431768211455) in
+             expr_let v8 := (uint128)(79228162514264337593543950335 *₂₅₆ v6 >> 128) in
+             expr_let v9 := ((uint128)(79228162514264337593543950335 *₂₅₆ v6) & 340282366920938463463374607431768211455) in
+             expr_let v10 := (uint128)(340282366841710300967557013911933812736 *₂₅₆ v7 >> 128) in
+             expr_let v11 := ((uint128)(340282366841710300967557013911933812736 *₂₅₆ v7) & 340282366920938463463374607431768211455) in
+             expr_let v12 := ADD_256 ((uint256)(v11 << 128), (uint256)(v9 << 128)) in
+             expr_let v13 := ADD_256 (79228162514264337593543950335 *₂₅₆ v7, v12₁) in
+             expr_let v14 := v13₂ +₁₂₈ v12₂ in
+             expr_let v15 := ADD_256 (v8, 340282366841710300967557013911933812736 *₂₅₆ v6) in
+             expr_let v16 := ADD_256 (v10, v15₁) in
+             expr_let v17 := ADD_256 (v14, v16₁) in
+             expr_let v18 := ADD_256 (v₁, v13₁) in
+             expr_let v19 := ADDC_256 (v18₂, v₂, v17₁) in
+             expr_let v20 := SELC (v19₂, 0, 115792089210356248762697446949407573530086143415290314195533631308867097853951) in
+             expr_let v21 := Z.cast uint256 @@ (fst @@ SUB_256 (v19₁, v20)) in
+             ADDM (v21, 0, 115792089210356248762697446949407573530086143415290314195533631308867097853951)
+     : Expr (type.type_primitive type.Z * type.type_primitive type.Z -> type.type_primitive type.Z)
+*)
 End Montgomery256.
 
 (* Extra-specialized ad-hoc pretty-printing *)
 Module Montgomery256PrintingNotations.
   Export ident.
-  Export BoundsAnalysis.ident.
-  Export BoundsAnalysis.type.Notations.
-  Export BoundsAnalysis.Indexed.expr.Notations.
-  Export BoundsAnalysis.ident.Notations.
-  Import BoundsAnalysis.type.
-  Import BoundsAnalysis.Indexed.expr.
-  Import BoundsAnalysis.ident.
-  Open Scope btype_scope.
+  Open Scope expr_scope.
+  Open Scope ctype_scope.
   Notation "'RegMod'" :=
-    (BoundsAnalysis.Indexed.expr.AppIdent
-                   (primitive {| BoundsAnalysis.type.value := 115792089210356248762697446949407573530086143415290314195533631308867097853951; BoundsAnalysis.type.value_bounded := _ |})
-                   BoundsAnalysis.Indexed.expr.TT) (only printing, at level 9) : nexpr_scope.
+    (AppIdent
+       (primitive 115792089210356248762697446949407573530086143415290314195533631308867097853951)
+       TT) (only printing, at level 9) : expr_scope.
   Notation "'RegPinv'" :=
-    (BoundsAnalysis.Indexed.expr.AppIdent
-                   (primitive {| BoundsAnalysis.type.value := 115792089210356248768974548684794254293921932838497980611635986753331132366849; BoundsAnalysis.type.value_bounded := _ |})
-                   BoundsAnalysis.Indexed.expr.TT) (only printing, at level 9) : nexpr_scope.
+    (AppIdent
+       (primitive 115792089210356248768974548684794254293921932838497980611635986753331132366849)
+       TT) (only printing, at level 9) : expr_scope.
   Notation "'RegZero'" :=
-    (BoundsAnalysis.Indexed.expr.AppIdent
-                   (primitive {| BoundsAnalysis.type.value := 0; BoundsAnalysis.type.value_bounded := _ |})
-                   BoundsAnalysis.Indexed.expr.TT) (only printing, at level 9) : nexpr_scope.
-  Notation "'$R'" := 115792089237316195423570985008687907853269984665640564039457584007913129639936 : nexpr_scope.
+    (AppIdent
+       (primitive 0)
+       TT) (only printing, at level 9) : expr_scope.
+  Notation "'$R'" := 115792089237316195423570985008687907853269984665640564039457584007913129639936 : expr_scope.
   Notation "'Lower128{RegMod}'" :=
-    (BoundsAnalysis.Indexed.expr.AppIdent
-                   (primitive {| BoundsAnalysis.type.value := 79228162514264337593543950335; BoundsAnalysis.type.value_bounded := _ |})
-                   BoundsAnalysis.Indexed.expr.TT) (only printing, at level 9) : nexpr_scope.
+    (AppIdent
+       (primitive 79228162514264337593543950335)
+       TT) (only printing, at level 9) : expr_scope.
   Notation "'RegMod' '<<' '128'" :=
-    (BoundsAnalysis.Indexed.expr.AppIdent
-                   (primitive {| BoundsAnalysis.type.value := 340282366841710300967557013911933812736; BoundsAnalysis.type.value_bounded := _ |})
-                   BoundsAnalysis.Indexed.expr.TT) (only printing, at level 9, format "'RegMod'  '<<'  '128'") : nexpr_scope.
+    (AppIdent
+       (primitive 340282366841710300967557013911933812736)
+       TT) (only printing, at level 9, format "'RegMod'  '<<'  '128'") : expr_scope.
   Notation "'Lower128{RegPinv}'" :=
-    (BoundsAnalysis.Indexed.expr.AppIdent
-                   (primitive {| BoundsAnalysis.type.value := 79228162514264337593543950337; BoundsAnalysis.type.value_bounded := _ |})
-                   BoundsAnalysis.Indexed.expr.TT) (only printing, at level 9) : nexpr_scope.
+    (AppIdent
+       (primitive 79228162514264337593543950337)
+       TT) (only printing, at level 9) : expr_scope.
   Notation "'RegPinv' '>>' '128'" :=
-    (BoundsAnalysis.Indexed.expr.AppIdent
-                   (primitive {| BoundsAnalysis.type.value := 340282366841710300986003757985643364352; BoundsAnalysis.type.value_bounded := _ |})
-                   BoundsAnalysis.Indexed.expr.TT) (only printing, at level 9, format "'RegPinv'  '>>'  '128'") : nexpr_scope.
+    (AppIdent
+       (primitive 340282366841710300986003757985643364352)
+       TT) (only printing, at level 9, format "'RegPinv'  '>>'  '128'") : expr_scope.
   Notation "'uint256'"
-    := (BoundsAnalysis.type.ZBounded 0 115792089237316195423570985008687907853269984665640564039457584007913129639935) : btype_scope.
+    := (r[0 ~> 115792089237316195423570985008687907853269984665640564039457584007913129639935]%zrange) : ctype_scope.
   Notation "'uint128'"
-    := (BoundsAnalysis.type.ZBounded 0 340282366920938463463374607431768211455) : btype_scope.
-  Notation "$r n" := (BoundsAnalysis.Indexed.expr.Var _ n) (at level 10, format "$r n") : nexpr_scope.
-  Notation "$r n '_lo'" := (fst @@ (BoundsAnalysis.Indexed.expr.Var (BoundsAnalysis.type.prod _ _) n))%nexpr (at level 10, format "$r n _lo") : nexpr_scope.
-  Notation "$r n '_hi'" := (snd @@ (BoundsAnalysis.Indexed.expr.Var (BoundsAnalysis.type.prod _ _) n))%nexpr (at level 10, format "$r n _hi") : nexpr_scope.
-  Notation "'c.Mul128x128(' '$r' n ',' x ',' y ');' f" :=
-    (expr_let n := mul _ _ uint256 @@ (x, y) in
-         f)%nexpr (at level 40, f at level 200, right associativity, format "'[' 'c.Mul128x128(' '$r' n ','  x ','  y ');' ']' '//' f") : nexpr_scope.
-  Notation "'c.Mul128x128(' '$r' n ',' x ',' y ')' '<<' count ';' f" :=
-    (expr_let n := shiftl _ _ count @@ (mul _ _ uint256 @@ (x, y)) in
-         f)%nexpr (at level 40, f at level 200, right associativity, format "'[' 'c.Mul128x128(' '$r' n ','  x ','  y ')'  '<<'  count ';' ']' '//' f") : nexpr_scope.
-  Notation "'c.Add256(' '$r' n ',' x ',' y ');' f" :=
-    (expr_let n := add_get_carry_concrete _ _ uint256 _ $R @@ (x, y) in
-         f)%nexpr (at level 40, f at level 200, right associativity, format "'[' 'c.Add256(' '$r' n ','  x ','  y ');' ']' '//' f") : nexpr_scope.
-  Notation "'c.Add128(' '$r' n ',' x ',' y ');' f" :=
-    (expr_let n := add_get_carry_concrete _ _ uint128 _ $R @@ (x, y) in
-         f)%nexpr (at level 40, f at level 200, right associativity, format "'[' 'c.Add128(' '$r' n ','  x ','  y ');' ']' '//' f") : nexpr_scope.
-  Notation "'c.Add64(' '$r' n ',' x ',' y ');' f" :=
-    (expr_let n := add _ _ uint128 @@ (x, y) in
-         f)%nexpr (at level 40, f at level 200, right associativity, format "'[' 'c.Add64(' '$r' n ','  x ','  y ');' ']' '//' f") : nexpr_scope.
-  Notation "'c.Addc(' '$r' n ',' x ',' y ');' f" :=
-    (expr_let n := add_with_get_carry_concrete _ _ _ uint256 _ $R @@ (_, x, y) in
-         f)%nexpr (at level 40, f at level 200, right associativity, format "'[' 'c.Addc(' '$r' n ','  x ','  y ');' ']' '//' f") : nexpr_scope.
-  Notation "'c.Selc(' '$r' n ',' y ',' z ');' f" :=
-    (expr_let n := zselect _ _ _ uint256 @@ (_, y, z) in
-         f)%nexpr (at level 40, f at level 200, right associativity, format "'[' 'c.Selc(' '$r' n ',' y ','  z ');' ']' '//' f") : nexpr_scope.
-  Notation "'c.Sub(' '$r' n ',' x ',' y ');' f" :=
-    (expr_let n := fst @@ (sub_get_borrow_concrete _ _ uint256 _ $R @@ (x, y)) in
-         f)%nexpr (at level 40, f at level 200, right associativity, format "'c.Sub(' '$r' n ','  x ','  y ');' '//' f") : nexpr_scope.
+    := (r[0 ~> 340282366920938463463374607431768211455]%zrange) : ctype_scope.
+  Notation "$ n" := (Var n) (at level 10, format "$ n") : expr_scope.
+  Notation "$ n" := (Z.cast _ @@ Var n) (at level 10, format "$ n") : expr_scope.
+  Notation "$ n '_lo'" := (fst @@ (Var n))%expr (at level 10, format "$ n _lo") : expr_scope.
+  Notation "$ n '_hi'" := (snd @@ (Var n))%expr (at level 10, format "$ n _hi") : expr_scope.
+  Notation "$ n '_lo'" := (Z.cast _ @@ (fst @@ (Var n)))%expr (at level 10, format "$ n _lo") : expr_scope.
+  Notation "$ n '_hi'" := (Z.cast _ @@ (snd @@ (Var n)))%expr (at level 10, format "$ n _hi") : expr_scope.
+  Notation "$ n '_lo'" := (Z.cast _ @@ (fst @@ (Z.cast2 _ @@ Var n)))%expr (at level 10, format "$ n _lo") : expr_scope.
+  Notation "$ n '_hi'" := (Z.cast _ @@ (snd @@ (Z.cast2 _ @@ Var n)))%expr (at level 10, format "$ n _hi") : expr_scope.
+  Notation "'c.Mul128x128(' '$' n ',' x ',' y ');' f" :=
+    (expr_let n := Z.cast uint256 @@ (Z.mul @@ (x, y)) in
+         f)%expr (at level 40, f at level 200, right associativity, format "'[' 'c.Mul128x128(' '$' n ','  x ','  y ');' ']' '//' f") : expr_scope.
+  Notation "'c.Mul128x128(' '$' n ',' x ',' y ')' '<<' count ';' f" :=
+    (expr_let n := Z.cast _ @@ (Z.shiftl count @@ (Z.cast uint256 @@ (Z.mul @@ (x, y)))) in
+         f)%expr (at level 40, f at level 200, right associativity, format "'[' 'c.Mul128x128(' '$' n ','  x ','  y ')'  '<<'  count ';' ']' '//' f") : expr_scope.
+  Notation "'c.Add256(' '$' n ',' x ',' y ');' f" :=
+    (expr_let n := Z.cast2 (uint256, _)%core @@ (Z.add_get_carry_concrete $R @@ (x, y)) in
+         f)%expr (at level 40, f at level 200, right associativity, format "'[' 'c.Add256(' '$' n ','  x ','  y ');' ']' '//' f") : expr_scope.
+  Notation "'c.Add128(' '$' n ',' x ',' y ');' f" :=
+    (expr_let n := Z.cast2 (uint128, _)%core @@ (Z.add_get_carry_concrete $R @@ (x, y)) in
+         f)%expr (at level 40, f at level 200, right associativity, format "'[' 'c.Add128(' '$' n ','  x ','  y ');' ']' '//' f") : expr_scope.
+  Notation "'c.Add64(' '$' n ',' x ',' y ');' f" :=
+    (expr_let n := Z.cast uint128 @@ (Z.add @@ (x, y)) in
+         f)%expr (at level 40, f at level 200, right associativity, format "'[' 'c.Add64(' '$' n ','  x ','  y ');' ']' '//' f") : expr_scope.
+  Notation "'c.Addc(' '$' n ',' x ',' y ');' f" :=
+    (expr_let n := Z.cast2 (uint256, _)%core @@ (Z.add_with_get_carry_concrete $R @@ (_, x, y)) in
+         f)%expr (at level 40, f at level 200, right associativity, format "'[' 'c.Addc(' '$' n ','  x ','  y ');' ']' '//' f") : expr_scope.
+  Notation "'c.Selc(' '$' n ',' y ',' z ');' f" :=
+    (expr_let n := Z.cast uint256 @@ (Z.zselect @@ (_, y, z)) in
+         f)%expr (at level 40, f at level 200, right associativity, format "'[' 'c.Selc(' '$' n ',' y ','  z ');' ']' '//' f") : expr_scope.
+  Notation "'c.Sub(' '$' n ',' x ',' y ');' f" :=
+    (expr_let n := Z.cast uint256 @@ (fst @@ (Z.cast2 (uint256, _)%core @@ (Z.sub_get_borrow_concrete $R @@ (x, y)))) in
+         f)%expr (at level 40, f at level 200, right associativity, format "'c.Sub(' '$' n ','  x ','  y ');' '//' f") : expr_scope.
   Notation "'c.AddM(' '$ret' ',' x ',' y ',' z ');'" :=
-    (add_modulo _ _ _ uint256 @@ (x, y, z))%nexpr (at level 40, format "'c.AddM(' '$ret' ','  x ','  y ','  z ');'") : nexpr_scope.
-  Notation "'c.ShiftR(' '$r' n ',' x ',' y ');' f" :=
-    (expr_let n := (shiftr _ _ y @@ x) in f)%nexpr (at level 40, f at level 200, right associativity, format "'[' 'c.ShiftR(' '$r' n ','  x ','  y ');' ']' '//' f") : nexpr_scope.
-  Notation "'c.ShiftL(' '$r' n ',' x ',' y ');' f" :=
-    (expr_let n := (shiftl _ _ y @@ x) in f)%nexpr (at level 40, f at level 200, right associativity, format "'[' 'c.ShiftL(' '$r' n ','  x ','  y ');' ']' '//' f") : nexpr_scope.
-  Notation "'c.Lower128(' '$r' n ',' x ');' f" :=
-    (expr_let n := (land _ _ 340282366920938463463374607431768211455 @@ x) in f)%nexpr (at level 40, f at level 200, right associativity, format "'[' 'c.Lower128(' '$r' n ','  x ');' ']' '//' f") : nexpr_scope.
+    (Z.cast uint256 @@ (Z.add_modulo @@ (x, y, z)))%expr (at level 40, format "'c.AddM(' '$ret' ','  x ','  y ','  z ');'") : expr_scope.
+  Notation "'c.ShiftR(' '$' n ',' x ',' y ');' f" :=
+    (expr_let n := Z.cast _ @@ (Z.shiftr y @@ x) in f)%expr (at level 40, f at level 200, right associativity, format "'[' 'c.ShiftR(' '$' n ','  x ','  y ');' ']' '//' f") : expr_scope.
+  Notation "'c.ShiftL(' '$' n ',' x ',' y ');' f" :=
+    (expr_let n := Z.cast _ @@ (Z.shiftl y @@ x) in f)%expr (at level 40, f at level 200, right associativity, format "'[' 'c.ShiftL(' '$' n ','  x ','  y ');' ']' '//' f") : expr_scope.
+  Notation "'c.Lower128(' '$' n ',' x ');' f" :=
+    (expr_let n := Z.cast _ @@ (Z.land 340282366920938463463374607431768211455 @@ x) in f)%expr (at level 40, f at level 200, right associativity, format "'[' 'c.Lower128(' '$' n ','  x ');' ']' '//' f") : expr_scope.
   Notation "'Lower128'"
-    := ((land uint256 uint128 340282366920938463463374607431768211455))
+    := (Z.cast uint128 @@ (Z.land 340282366920938463463374607431768211455))
          (at level 10, only printing, format "Lower128")
-  : nexpr_scope.
+  : expr_scope.
   Notation "( v << count )"
-    := ((shiftl _ _ count @@ v)%nexpr)
+    := (Z.cast _ @@ (Z.shiftl count @@ v)%expr)
          (format "( v  <<  count )")
-       : nexpr_scope.
+       : expr_scope.
   Notation "( x >> count )"
-    := ((shiftr _ _ count @@ x)%nexpr)
+    := (Z.cast _ @@ (Z.shiftr count @@ x)%expr)
          (format "( x  >>  count )")
-       : nexpr_scope.
+       : expr_scope.
+  Notation "x * y"
+    := (Z.cast uint256 @@ (Z.mul @@ (x, y)))
+       : expr_scope.
 End Montgomery256PrintingNotations.
 
 Import Montgomery256PrintingNotations.
-Local Open Scope nexpr_scope.
+Local Open Scope expr_scope.
 
 
 Print Montgomery256.montred256.
 (*
-c.ShiftR($r3, $r1_lo, 128);
-c.Lower128($r4, $r1_lo);
-c.Mul128x128($r5, $r3, Lower128{RegPinv});
-c.Lower128($r7, $r5);
-c.Mul128x128($r8, $r4, RegPinv >> 128);
-c.Lower128($r10, $r8);
-c.ShiftL($r11, $r10, 128);
-c.ShiftL($r12, $r7, 128);
-c.Mul128x128($r17, $r4, Lower128{RegPinv});
-c.Add128($r18, $r11, $r12);
-c.Add256($r19, $r17, $r18_lo);
-c.ShiftR($r43, $r19_lo, 128);
-c.Lower128($r44, $r19_lo);
-c.Mul128x128($r45, $r43, Lower128{RegMod});
-c.ShiftR($r46, $r45, 128);
-c.Lower128($r47, $r45);
-c.Mul128x128($r48, $r44, RegMod << 128);
-c.ShiftR($r49, $r48, 128);
-c.Lower128($r50, $r48);
-c.ShiftL($r51, $r50, 128);
-c.ShiftL($r52, $r47, 128);
-c.Mul128x128($r57, $r44, Lower128{RegMod});
-c.Add128($r58, $r51, $r52);
-c.Add256($r59, $r57, $r58_lo);
-c.Add64($r60, $r59_hi, $r58_hi);
-c.Mul128x128($r67, $r43, RegMod << 128);
-c.Add256($r69, $r46, $r67);
-c.Add256($r70, $r49, $r69_lo);
-c.Add256($r80, $r60, $r70_lo);
-c.Add256($r83, $r1_lo, $r59_lo);
-c.Addc($r84, $r1_hi, $r80_lo);
-c.Selc($r85,RegZero, RegMod);
-c.Sub($r86, $r84_lo, $r85);
-c.AddM($ret, $r86, RegZero, RegMod);
-     : expr uint256
+c.ShiftR($v0, $v_lo, 128);
+c.Lower128($v1, $v_lo);
+c.Lower128($v2, Lower128{RegPinv} * $v0);
+c.Lower128($v3, RegPinv >> 128 * $v1);
+c.Add256($v4, ($v3 << 128), ($v2 << 128));
+c.Add256($v5, Lower128{RegPinv} * $v1, $v4_lo);
+c.ShiftR($v6, $v5_lo, 128);
+c.Lower128($v7, $v5_lo);
+c.ShiftR($v8, Lower128{RegMod} * $v6, 128);
+c.Lower128($v9, Lower128{RegMod} * $v6);
+c.ShiftR($v10, RegMod << 128 * $v7, 128);
+c.Lower128($v11, RegMod << 128 * $v7);
+c.Add256($v12, ($v11 << 128), ($v9 << 128));
+c.Add256($v13, Lower128{RegMod} * $v7, $v12_lo);
+c.Add64($v14, $v13_hi, $v12_hi);
+c.Add256($v15, $v8, RegMod << 128 * $v6);
+c.Add256($v16, $v10, $v15_lo);
+c.Add256($v17, $v14, $v16_lo);
+c.Add256($v18, $v_lo, $v13_lo);
+c.Addc($v19, $v_hi, $v17_lo);
+c.Selc($v20,RegZero, RegMod);
+c.Sub($v21, $v19_lo, $v20);
+c.AddM($ret, $v21, RegZero, RegMod);
+     : Expr
+         (type.type_primitive type.Z * type.type_primitive type.Z ->
+          type.type_primitive type.Z)
  *)
